Implemented structures for protocol parameters and token bundles.

src/Ledger/Costing.lean
@@ -1,38 +1,38 @@
 
-import Ledger.ProtocolParameters
+import Ledger.Protocol
 import Ledger.Sizing
 
 
--- Computations for costs on the ledger..
+-- Computations for costs on the ledger.
 namespace Ledger.Costing
 
 
-open Ledger.ProtocolParameters (txFeeFixed txFeePerByte utxoCostPerWord)
-open Ledger.Sizing             (utxoEntrySize)
+open Ledger.Protocol (ProtocolParameters)
+open Ledger.Sizing   (TokenBundle utxoEntrySize)
 
 
 -- Compute the minimum Ada for a UTxO.
-def minimumAda (hasDatum : Bool) (numPolicies numAssets sumAssetNameLengths : Nat) : Nat :=
-  utxoCostPerWord
-    * utxoEntrySize hasDatum numPolicies numAssets sumAssetNameLengths
+def minimumAda (pp : ProtocolParameters) (hasDatum : Bool) (tb : TokenBundle) : Nat :=
+  pp.utxoCostPerWord * utxoEntrySize hasDatum tb
 
 
 -- | Compare to output of `cardano-cli` during Epoch 330.
-example : minimumAda false  0   0          0 =   999978 := rfl
-example : minimumAda false  1   1          1 =  1344798 := rfl
-example : minimumAda false  1   1         32 =  1448244 := rfl
-example : minimumAda false  1 110 (110 * 32) = 22137444 := rfl
-example : minimumAda false 60  60 ( 60 * 32) = 19758186 := rfl
-example : minimumAda true   0   0          0 =  1344798 := rfl
-example : minimumAda true   1   1          1 =  1689618 := rfl
-example : minimumAda true   2   2          4 =  1862028 := rfl
+example : minimumAda default false {numPolicies :=  0, numAssets :=   0, sumAssetNameLengths :=        0} =   999978 := rfl
+example : minimumAda default false {numPolicies :=  1, numAssets :=   1, sumAssetNameLengths :=        1} =  1344798 := rfl
+example : minimumAda default false {numPolicies :=  1, numAssets :=   1, sumAssetNameLengths :=       32} =  1448244 := rfl
+example : minimumAda default false {numPolicies :=  1, numAssets := 110, sumAssetNameLengths := 110 * 32} = 22137444 := rfl
+example : minimumAda default false {numPolicies := 60, numAssets :=  60, sumAssetNameLengths :=  60 * 32} = 19758186 := rfl
+example : minimumAda default true  {numPolicies :=  0, numAssets :=   0, sumAssetNameLengths :=        0} =  1344798 := rfl
+example : minimumAda default true  {numPolicies :=  1, numAssets :=   1, sumAssetNameLengths :=        1} =  1689618 := rfl
+example : minimumAda default true  {numPolicies :=  2, numAssets :=   2, sumAssetNameLengths :=        4} =  1862028 := rfl
 
 
 -- Fee in Lovelace for a transaction of a specified size.
-def feeForBytes (bytes : Nat) : Nat :=  txFeeFixed + bytes * txFeePerByte
+def feeForBytes (pp : ProtocolParameters) (bytes : Nat) : Nat :=
+  pp.txFeeFixed + bytes * pp.txFeePerByte
 
-example : feeForBytes    0 = 155381         := rfl
-example : feeForBytes 1000 = 155381 + 44000 := rfl
+example : feeForBytes default    0 = 155381         := rfl
+example : feeForBytes default 1000 = 155381 + 44000 := rfl
 
 
 end Ledger.Costing
