src/Ledger/Protocol.lean
@@ -1,0 +1,58 @@
+
+-- Protocol parameters.
+namespace Ledger.Protocol
+
+
+structure ProtocolParameters :=
+
+  -- Required Lovelace for each word in a UTxO.
+  utxoCostPerWord : Nat
+
+  -- Lovelace fee per transaction.
+  txFeeFixed : Nat
+
+  -- Additional lovelace fee per byte.
+  txFeePerByte : Nat
+
+  -- The maximum value size in bytes.
+  maxValueSize : Nat
+
+  -- Maximum transaction size in bytes.
+  maxTxSize : Nat
+
+  -- The maximum number of collateral inputs.
+  maxCollateralInputs : Nat
+
+  -- The collateral percentage relative to the fee.
+  collateralPercentage : Float
+
+  -- The maximum execution memory allowed for a transaction.
+  maxTxExecutionMemory : Nat
+
+  -- The maximum execution steps allowed for a transaction.
+  maxTxExecutionSteps : Nat
+
+  -- The maximum execution memory allowed for a transaction.
+  executionMemoryPrice : Float
+
+  -- The maximum execution steps allowed for a transaction.
+  executionStepsPrice : Float
+
+
+instance : Inhabited ProtocolParameters where
+  default := {
+    utxoCostPerWord      := 34482
+    txFeeFixed           := 155381
+    txFeePerByte         := 44
+    maxTxSize            := 16384
+    maxValueSize         := 5000
+    maxCollateralInputs  := 3
+    collateralPercentage := 150
+    maxTxExecutionMemory := 16000000
+    maxTxExecutionSteps  := 10000000000
+    executionMemoryPrice := 5.77e-2
+    executionStepsPrice  := 7.21e-5
+  }   
+
+
+end Ledger.Protocol
